Prove the naturality of the materialization with respect to the equivalences.

RegexCorrectness/NFA/Semantics/Equivalence/Basic.lean
@@ -8,9 +8,32 @@ namespace Regex.NFA
 
 inductive EquivUpdate : CaptureGroups → List (Nat × String.Pos) → Prop where
   | empty : EquivUpdate .empty []
-  | group {groups updates tag first last} (h : EquivUpdate groups updates) :
+  | group {groups updates tag first last} (eqv : EquivUpdate groups updates) :
     EquivUpdate (.group tag first last groups) ((2 * tag, first) :: updates ++ [(2 * tag + 1, last)])
-  | concat {groups₁ groups₂ updates₁ updates₂} (h₁ : EquivUpdate groups₁ updates₁) (h₂ : EquivUpdate groups₂ updates₂) :
+  | concat {groups₁ groups₂ updates₁ updates₂} (eqv₁ : EquivUpdate groups₁ updates₁) (eqv₂ : EquivUpdate groups₂ updates₂) :
     EquivUpdate (.concat groups₁ groups₂) (updates₁ ++ updates₂)
+
+theorem EquivUpdate.mem_groups_of_mem_updates {groups updates offset pos}
+  (h : (offset, pos) ∈ updates) (eqv : EquivUpdate groups updates) :
+  ∃ tag first last, (tag, first, last) ∈ groups ∧ (offset = 2 * tag ∨ offset = 2 * tag + 1) := by
+  induction eqv with
+  | empty => simp at h
+  | @group groups updates tag first last eqv ih =>
+    simp at h
+    match h with
+    | .inl eq => exact ⟨tag, first, last, by simp, by simp [eq]⟩
+    | .inr (.inl mem) =>
+      have ⟨tag, first, last, mem, eq⟩ := ih mem
+      exact ⟨tag, first, last, by simp [mem], eq⟩
+    | .inr (.inr eq) => exact ⟨tag, first, last, by simp, by simp [eq]⟩
+  | @concat groups₁ groups₂ updates₁ updates₂ eqv₁ eqv₂ ih₁ ih₂ =>
+    simp at h
+    cases h with
+    | inl mem =>
+      have ⟨tag, first, last, mem, eq⟩ := ih₁ mem
+      exact ⟨tag, first, last, by simp [mem], eq⟩
+    | inr mem =>
+      have ⟨tag, first, last, mem, eq⟩ := ih₂ mem
+      exact ⟨tag, first, last, by simp [mem], eq⟩
 
 end Regex.NFA
