RegexCorrectness/VM/Correspondence/Materialize/Naturality.lean
@@ -1,0 +1,116 @@
+import RegexCorrectness.Data.Expr.Semantics
+import RegexCorrectness.NFA.Semantics.Equivalence
+import RegexCorrectness.VM.Correspondence.Materialize.Lemmas
+
+set_option autoImplicit false
+
+open Regex.Data (Vec Expr)
+open String (Pos)
+
+namespace Regex.NFA
+
+/--
+Under suitable conditions, the equivalence between capture groups and NFA buffer updates can be
+naturally transformed into a materialized version.
+-/
+theorem EquivUpdate.materialize {e : Expr} {n span span' groups updates}
+  (c : e.Captures span span' groups) (disj : e.Disjoint)
+  (eqv : EquivUpdate groups updates) :
+  EquivMaterializedUpdate (materializeRegexGroups groups) (materializeUpdates n updates) := by
+  induction c generalizing updates with
+  | char | sparse | epsilon | starEpsilon =>
+    cases eqv with
+    | empty => simp [EquivMaterializedUpdate]
+  | @group span span' groups tag e c ih =>
+    simp [Expr.Disjoint] at disj
+    cases eqv with
+    | @group groups updates _ _ _ eqv =>
+      have ih := ih disj.2 eqv
+      simp [materializeUpdates]
+      rw [materializeUpdatesAux_cons_of_not_in ?_]
+      . simp [materializeUpdatesAux_snoc]
+        intro tag'
+        simp
+        apply And.intro
+        . intro h₁
+          if h : tag = tag' then
+            simp [h]
+          else
+            have h' : 2 * tag ≠ 2 * tag' := by omega
+            have h'' : 2 * tag + 1 ≠ 2 * tag' := by omega
+            simp [h, h', h'']
+            exact (ih tag').1 h₁
+        . intro h₂
+          if h : tag = tag' then
+            simp [h]
+          else
+            have h' : 2 * tag ≠ 2 * tag' + 1 := by omega
+            have h'' : 2 * tag + 1 ≠ 2 * tag' + 1 := by omega
+            simp [h, h', h'']
+            exact (ih tag').2 h₂
+      . intro offset pos mem
+        simp at mem
+        cases mem with
+        | inl mem =>
+          have ⟨tag', first, last, mem', eq⟩ := eqv.mem_groups_of_mem_updates mem
+          cases eq with
+          | inl eq =>
+            suffices tag ≠ tag' by omega
+            intro eq
+            subst tag'
+            have mem_tags := c.mem_tags_of_mem_groups tag first last mem'
+            exact disj.1 mem_tags
+          | inr eq => omega
+        | inr eq => omega
+  | alternateLeft _ ih =>
+    simp [Expr.Disjoint] at disj
+    exact ih disj.2.1 eqv
+  | alternateRight _ ih =>
+    simp [Expr.Disjoint] at disj
+    exact ih disj.2.2 eqv
+  | concat _ _ ih₁ ih₂ =>
+    simp [Expr.Disjoint] at disj
+    cases eqv with
+    | @concat _ _ update₁ update₂ eqv₁ eqv₂ =>
+      have ih₁ := ih₁ disj.2.1 eqv₁
+      have ih₂ := ih₂ disj.2.2 eqv₂
+      exact concat ih₁ ih₂
+  | starConcat _ _ ih₁ ih₂ =>
+    simp [Expr.Disjoint] at disj
+    cases eqv with
+    | @concat _ _ update₁ update₂ eqv₁ eqv₂ =>
+      have ih₁ := ih₁ disj eqv₁
+      have ih₂ := ih₂ (by simp [Expr.Disjoint, disj]) eqv₂
+      exact concat ih₁ ih₂
+where
+  concat {g₁ g₂ u₁ u₂}
+    (eqv₁ : EquivMaterializedUpdate (materializeRegexGroups g₁) (materializeUpdates n u₁))
+    (eqv₂ : EquivMaterializedUpdate (materializeRegexGroups g₂) (materializeUpdates n u₂)) :
+    EquivMaterializedUpdate (materializeRegexGroups (.concat g₁ g₂)) (materializeUpdates n (u₁ ++ u₂)) := by
+    intro tag
+    apply And.intro
+    . intro h₁
+      simp [materializeUpdates_append_getElem]
+      match h : materializeRegexGroups g₂ tag with
+      | .some (first, last) =>
+        have := (eqv₂ tag).1 h₁
+        simp [h] at this
+        simp [←this]
+      | .none =>
+        have := (eqv₂ tag).1 h₁
+        simp [h] at this
+        simp [←this, (eqv₁ tag).1 h₁]
+    . intro h₂
+      simp [materializeUpdates_append_getElem]
+      match h : materializeRegexGroups g₂ tag with
+      | .some (first, last) =>
+        have := (eqv₂ tag).2 h₂
+        simp [h] at this
+        simp [←this]
+      | .none =>
+        have := (eqv₂ tag).2 h₂
+        simp [h] at this
+        simp [←this, (eqv₁ tag).2 h₂]
+
+
+end Regex.NFA
